명확하게 다른 '생성자' 만, 확실하게 다르다...! 으으

src/lean/Nemonuri/Property.lean
@@ -1,7 +1,5 @@
 module
 
-public import Mathlib.Tactic.Contrapose
-public import Mathlib.Logic.Basic
 
 @[expose] public section public_s
 
@@ -10,18 +8,17 @@ universe u
 
 namespace Nemonuri
 
-structure Property (σ: Type u) where
-  protected T: Type u
-  protected v: σ → T
+--structure Property (σ: Type u) (T: Type u) where
+--  v: σ → T
 
-namespace Property
+--namespace Property
 
-class ZeroEq {σ: Type u} [Zero σ] (p: Property σ) [Zero p.T] : Prop where
-  zero_eq: (p.v 0 = 0)
+class ZeroEq {σ T: Type u} [Zero σ] [Zero T] (f: σ → T) : Prop where
+  zero_eq: (f 0 = 0)
 
-variable {σ: Type u} [Zero σ] (p: Property σ) [Zero p.T]
+variable {σ T: Type u} [Zero σ] [Zero T] (f: σ → T)
 
-theorem zeroEq_iff : (ZeroEq p) ↔ (p.v 0 = 0) := by
+theorem zeroEq_iff : (ZeroEq f) ↔ (f 0 = 0) := by
   constructor
   · intro h
     obtain ⟨h'⟩ := h ; exact h'
@@ -29,38 +26,19 @@ theorem zeroEq_iff : (ZeroEq p) ↔ (p.v 0 = 0) := by
     constructor ; exact h
 
 class SourceExists : Prop where
-  source_exists (v: p.T) (h: v ≠ 0) : ∃(s: σ), (p.v s = v)
+  source_exists (v: T) (h: v ≠ 0) : ∃(s: σ), (f s = v)
 
 omit [Zero σ] in
-theorem sourceExists_iff : (SourceExists p) ↔ ((v: p.T) → (v ≠ 0) → ∃(s: σ), (p.v s = v)) := by
+theorem sourceExists_iff : (SourceExists f) ↔ ((v: T) → (v ≠ 0) → ∃(s: σ), (f s = v)) := by
   constructor
   · intro h
     obtain ⟨h'⟩ := h ; exact h'
   · intro h
     constructor ; exact h
 
-class abbrev IsLawfulPartial : Prop := ZeroEq p, SourceExists p
 
+class abbrev IsProperty : Prop := ZeroEq f, SourceExists f
 
-end Property
-
-
-class PartialProperty (σ: Type u) [Zero σ]
-  extends
-    toProperty: Property σ
-  where
-  protected zero : T
-  is_lawful_partial : @Property.IsLawfulPartial _ _ toProperty ⟨zero⟩
-
-variable {σ: Type u} [Zero σ] [pp: PartialProperty σ]
-
-instance PartialProperty.instZeroT : Zero pp.T where
-  zero := pp.zero
-
-open Property in
-instance PartialProperty.instIsLawfulPartial : IsLawfulPartial pp.toProperty where
-  zero_eq := pp.is_lawful_partial.zero_eq
-  source_exists := pp.is_lawful_partial.source_exists
 
 
 end Nemonuri
